Hybrid_Programs/Verification_Examples/Hoare_Help.thy
@@ -1,0 +1,251 @@
+theory Hoare_Help
+
+imports
+  "Hybrid-Verification.Diff_Dyn_Logic"
+begin
+
+lemma hoare_kcomp_inv_rhs:
+  assumes "\<^bold>{P\<^bold>} G \<^bold>{Q\<^bold>}" and "\<^bold>{Q\<^bold>} F \<^bold>{Q\<^bold>}"
+  shows "\<^bold>{P\<^bold>} G ; F \<^bold>{Q\<^bold>}"
+  using assms hoare_kcomp by blast
+
+lemma hoare_stengthen_post:
+  assumes "\<^bold>{P\<^bold>} G \<^bold>{Q\<^bold>}" and "`Q \<longrightarrow> R`"
+  shows "\<^bold>{P\<^bold>} G \<^bold>{R\<^bold>}"
+  using assms Diff_Dyn_Logic.strengthen by blast
+
+lemma strenghten_pre_post:
+  assumes "\<^bold>{P\<^bold>} F \<^bold>{Q\<^bold>}"
+  shows "\<^bold>{P \<and> \<guillemotleft>I\<guillemotright>\<^bold>} F \<^bold>{Q \<and> \<guillemotleft>I\<guillemotright>\<^bold>}"
+  using assms fbox_def by auto
+
+lemma hoare_do_while:
+  assumes "\<^bold>{I\<^bold>} A \<^bold>{I \<and> T\<^bold>}" and "\<^bold>{I \<and> T\<^bold>} X \<^bold>{I\<^bold>}"
+  shows "\<^bold>{I\<^bold>} (A ; WHILE T DO X) \<^bold>{\<not> T \<and> I\<^bold>}"
+  using assms
+  by (metis (mono_tags) hoare_conj_pos hoare_kcomp hoare_while)
+
+lemma nondet_choice_commute: "P \<sqinter> Q = Q \<sqinter> P"
+  unfolding nondet_choice_def by auto
+
+lemma kcomp_right_dist_nondetchoice:
+  "(P \<sqinter> Q) ; R = (P ; R) \<sqinter> (Q ; R)"
+  unfolding nondet_choice_def kcomp_def
+  by (auto, metis UN_Un comp_apply)
+
+lemma kcomp_left_dist_nondetchoice:
+  "P ; (Q \<sqinter> R) = (P ; Q) \<sqinter> (P ; R)"
+  unfolding nondet_choice_def kcomp_def 
+  by (auto, metis UN_Un_distrib comp_apply)
+
+lemma kcomp_left_dist_Nondet_choice: "(\<Sqinter>i\<in>UNIV. P ; F P i) = P ; (\<Sqinter>i\<in>UNIV. F P i)"
+  unfolding Nondet_choice_def kcomp_def apply auto
+  by fastforce
+
+lemma test_False:
+  "\<questiondown>False? = abort"
+  unfolding test_def abort_def by auto
+
+lemma While_False_eq_skip:
+  "WHILE False DO X = skip"
+  unfolding kcomp_def while_def test_def skip_def
+  by (auto, metis UN_singleton comp_apply kstar_empty)
+
+lemma abort_skip_eq_skip: "abort \<sqinter> skip = skip"
+  unfolding abort_def nondet_choice_def skip_def by auto
+
+lemma kstar_one_or_zero_or_more: "P\<^sup>* = P \<sqinter> P\<^sup>*"
+  unfolding nondet_choice_def kstar_def apply auto
+  apply (simp add:fun_eq_iff, auto)
+  by (metis kpower_Suc_0)
+
+lemma 
+  assumes "i > 0"
+  shows "kpower P i = P ; (kpower P (i-1))"
+  using assms unfolding kpower_def skip_def oops
+
+lemma "(\<Sqinter>i\<in>UNIV-{0}. kpower P i) = (P ; P\<^sup>*)"
+  unfolding Nondet_choice_def nondet_choice_def kstar_def kcomp_def apply auto
+  oops
+
+lemma
+  assumes "xa \<in> kpower P i x" "\<forall>n. \<forall>z\<in>(P x). xa \<notin> kpower P n z"
+  shows "xa = x"
+  apply (insert assms) unfolding kpower_def
+  oops
+
+lemma UNIV_kpower_skip_nondet_choice:"(\<Sqinter>i\<in>UNIV. kpower P i) = skip \<sqinter> (\<Sqinter>i\<in>UNIV. (kpower P i ; P))"
+  unfolding Nondet_choice_def nondet_choice_def skip_def kcomp_def
+  apply (simp add:fun_eq_iff)
+  apply (safe, auto)
+  defer
+    apply (metis insertI1 kpower_0)
+   apply (metis (mono_tags, opaque_lifting) UN_I comp_apply kcomp_def kpower_Suc')
+  by (metis (no_types, opaque_lifting) UN_E comp_apply kcomp_def kpower_0 kpower_Suc' not0_implies_Suc singletonD)
+
+lemma UNIV_kpower_skip_nondet_choice':"(\<Sqinter>i\<in>UNIV. kpower P i) = skip \<sqinter> (\<Sqinter>i\<in>UNIV. P ; kpower P i)"
+proof -
+  have "(\<Sqinter>i\<in>UNIV. kpower P i) = skip \<sqinter> (\<Sqinter>i\<in>UNIV. (kpower P i ; P))"
+    using UNIV_kpower_skip_nondet_choice
+    by blast
+  also have "... = skip \<sqinter> (\<Sqinter>i\<in>UNIV. (P ; kpower P i))"
+    using kcomp_kpower
+    by metis
+  then show ?thesis using calculation by auto
+qed
+
+lemma UNIV_kpower_skip_one_more: "(\<Sqinter>i\<in>UNIV. kpower P i) = skip \<sqinter> P ; (\<Sqinter>i\<in>UNIV. kpower P i)"
+  using kcomp_left_dist_Nondet_choice UNIV_kpower_skip_nondet_choice' by metis
+
+lemma kstar_zero_or_one_or_more: "P\<^sup>* = skip \<sqinter> (P ; P\<^sup>*)"
+  by (metis UNIV_kpower_skip_one_more kstar_alt)
+
+lemma "(\<questiondown>\<not> T? ; X)\<^sup>* = skip \<sqinter> \<questiondown>\<not> T? ; X ; (\<questiondown>\<not> T? ; X)\<^sup>*"
+  using kstar_zero_or_one_or_more by blast 
+
+lemma test_not_kcomp_test_abort: "(\<questiondown>\<not> T? ; \<questiondown>T?) = abort"
+  unfolding test_def kcomp_def abort_def by auto
+
+lemma kcomp_left_zero: "abort ; X = abort"
+  unfolding abort_def kcomp_def by auto
+
+lemma nondet_choice_abort_unit: "P \<sqinter> abort = P"
+  by (simp add: abort_def nondet_choice_def)
+
+lemma negative_test_WHILE_DO_absorb:"(\<questiondown>\<not> T? ; WHILE T DO X) = \<questiondown>\<not> T?"
+proof -
+  have "\<questiondown>\<not> T? ; WHILE T DO X = \<questiondown>\<not> T? ; (\<questiondown>T? ; X)\<^sup>* ; \<questiondown>\<not> T?"
+    unfolding while_def
+    by (simp add: kcomp_assoc)
+  also have "... = \<questiondown>\<not> T? ; ((skip \<sqinter> (\<questiondown>T? ; X) ; (\<questiondown>T? ; X)\<^sup>*) ; \<questiondown>\<not> T?)"
+    using kstar_zero_or_one_or_more
+    by (metis kcomp_assoc)
+  also have "... = (\<questiondown>\<not> T? ; (skip \<sqinter> (\<questiondown>T? ; X) ; (\<questiondown>T? ; X)\<^sup>*)) ; \<questiondown>\<not> T?"
+    by (metis kcomp_assoc)
+  also have "... = ((\<questiondown>\<not> T? ; skip) \<sqinter> (\<questiondown>\<not> T? ; (\<questiondown>T? ; X) ; (\<questiondown>T? ; X)\<^sup>*)) ; \<questiondown>\<not> T?"
+    by (simp add: kcomp_assoc kcomp_left_dist_nondetchoice)
+  also have "... = (\<questiondown>\<not> T? \<sqinter> (\<questiondown>\<not> T? ; (\<questiondown>T? ; X) ; (\<questiondown>T? ; X)\<^sup>*)) ; \<questiondown>\<not> T?"
+    by (simp add: kcomp_skip(1))
+  also have "... = (\<questiondown>\<not> T? \<sqinter> ((\<questiondown>\<not> T? ; \<questiondown>T?) ; X) ; (\<questiondown>T? ; X)\<^sup>*) ; \<questiondown>\<not> T?"
+    by (metis kcomp_assoc)
+  also have "... = (\<questiondown>\<not> T? \<sqinter> (abort ; X) ; (\<questiondown>T? ; X)\<^sup>*) ; \<questiondown>\<not> T?"
+    using test_not_kcomp_test_abort by metis
+  also have "... = (\<questiondown>\<not> T? \<sqinter> abort) ; \<questiondown>\<not> T?"
+    using kcomp_left_zero by metis
+  also have "... = \<questiondown>\<not> T? ; \<questiondown>\<not> T?"
+    using nondet_choice_abort_unit by metis
+  also have "... = \<questiondown>\<not> T?"
+    unfolding test_def kcomp_def by auto
+  finally show ?thesis .
+qed
+
+lemma WHILE_unroll:
+  "WHILE T DO X = \<questiondown>\<not> T? \<sqinter> (\<questiondown>T? ; X) ; WHILE T DO X"
+proof -
+  have while_T_do_X:"WHILE T DO X = (\<questiondown>T? ; X)\<^sup>* ; \<questiondown>\<not> T?"
+    unfolding while_def by auto
+  also have "... = (skip \<sqinter> (\<questiondown>T? ; X) ; (\<questiondown>T? ; X)\<^sup>*) ; \<questiondown>\<not> T?"
+    using kstar_zero_or_one_or_more by metis
+  also have "... = (skip ; \<questiondown>\<not> T?) \<sqinter> (\<questiondown>T? ; X) ; (\<questiondown>T? ; X)\<^sup>* ; \<questiondown>\<not> T?"
+    using kcomp_right_dist_nondetchoice by blast
+  also have "... = \<questiondown>\<not> T? \<sqinter> (\<questiondown>T? ; X) ; (\<questiondown>T? ; X)\<^sup>* ; \<questiondown>\<not> T?"
+    by (simp add: kcomp_skip(2))
+  also have "... = \<questiondown>\<not> T? \<sqinter> (\<questiondown>T? ; X) ; WHILE T DO X"
+    by (simp add: kcomp_assoc while_T_do_X)
+  finally show ?thesis .
+qed
+  
+lemma WHILE_unroll_IF: "IF T THEN X ELSE skip ; WHILE T DO X = WHILE T DO X"
+proof -
+  have "IF T THEN X ELSE skip ; WHILE T DO X = (\<questiondown>T? ; X \<sqinter> \<questiondown>\<not> T? ; skip) ; WHILE T DO X"
+    by (simp add:if_then_else_eq)
+  also have "... = (\<questiondown>T? ; X ; WHILE T DO X) \<sqinter> (\<questiondown>\<not> T? ; skip ; WHILE T DO X)"
+    using kcomp_right_dist_nondetchoice by blast
+  also have "... = (\<questiondown>T? ; X ; WHILE T DO X) \<sqinter> (\<questiondown>\<not> T? ; WHILE T DO X)"
+    by (simp add: kcomp_skip(1))
+  also have "... = (\<questiondown>T? ; X ; WHILE T DO X) \<sqinter> \<questiondown>\<not> T?"
+    using negative_test_WHILE_DO_absorb by metis
+  also have "... = \<questiondown>\<not> T? \<sqinter> (\<questiondown>T? ; X ; WHILE T DO X)"
+    using nondet_choice_commute by auto
+  also have "... = WHILE T DO X"
+    using WHILE_unroll by metis
+  finally show ?thesis .
+qed
+
+lemma hoare_if_then_else:
+  assumes "\<^bold>{P\<^bold>} X \<^bold>{Q\<^bold>}" "\<^bold>{P\<^bold>} Y \<^bold>{Q\<^bold>}"
+  shows "\<^bold>{P\<^bold>} IF T THEN X ELSE Y \<^bold>{Q\<^bold>}"
+  using assms 
+  by fastforce
+
+lemma hoare_if_then_cond:
+  assumes "`P \<longrightarrow> T`" "\<^bold>{P\<^bold>} X \<^bold>{Q\<^bold>}"
+  shows "\<^bold>{P\<^bold>} IF T THEN X ELSE Y \<^bold>{Q\<^bold>}"
+  using assms unfolding fbox_def ifthenelse_def 
+  by (auto simp add: taut_def)
+
+lemma hoare_weaken_pre_conj:
+  assumes "`Q \<longrightarrow> P`" "\<^bold>{P \<and> Q\<^bold>} X \<^bold>{R\<^bold>}" 
+  shows "\<^bold>{Q\<^bold>} X \<^bold>{R\<^bold>}"
+  using assms
+  by (simp add: refine_iff_implies taut_def)
+
+lemma hoare_strengthen_post:
+  assumes "`T \<longrightarrow> R`" "\<^bold>{P\<^bold>} X \<^bold>{R \<and> T\<^bold>}" 
+  shows "\<^bold>{P\<^bold>} X \<^bold>{R\<^bold>}"
+  using assms
+  by (simp add: hoare_conj_pos)
+  
+lemma hoare_strengthen_pos_universal:
+  assumes "`U`" "\<^bold>{P\<^bold>} X \<^bold>{R\<^bold>}" 
+  shows "\<^bold>{P\<^bold>} X \<^bold>{U \<and> R\<^bold>}"
+  using assms 
+  by (simp add: refine_iff_implies taut_def)
+
+
+lemma
+  shows "\<^bold>{P\<^bold>} skip \<^bold>{Q\<^bold>}"
+  nitpick
+  oops
+
+lemma nmods_while:
+  assumes "X nmods e"
+  shows "WHILE T DO X nmods e"
+  using assms unfolding while_def
+  apply auto
+  apply (rule nmods_seq) 
+   apply (rule nmods_star)
+   apply (rule nmods_seq)
+  by (rule nmods_test, simp, rule nmods_test)
+
+lemma nmods_subset:
+  assumes "P nmods I" "\<forall>s. Q s \<subseteq> P s"
+  shows "Q nmods I"
+  by (meson assms(1) assms(2) not_modifies_def subsetD)
+
+lemma nmods_frame_law':
+  assumes "S nmods I" "\<^bold>{P \<and> I\<^bold>} S \<^bold>{Q\<^bold>}"
+  shows "\<^bold>{P \<and> I\<^bold>} S \<^bold>{Q \<and> I\<^bold>}"
+  using assms
+  by (auto simp add: prog_defs fbox_def expr_defs not_modifies_def)
+
+lemma hoare_while_unroll_kcomp:
+  assumes "\<^bold>{P\<^bold>} IF T THEN X ELSE skip \<^bold>{Q\<^bold>}" "\<^bold>{Q\<^bold>} WHILE T DO X \<^bold>{R\<^bold>}" 
+  shows "\<^bold>{P\<^bold>} WHILE T DO X \<^bold>{R\<^bold>}"
+  using assms WHILE_unroll_IF
+  by (metis hoare_kcomp) 
+
+(*
+  by (metis (mono_tags) SEXP_def hoare_kcomp nmods_invariant not_modifies_def)
+  by (metis (mono_tags) hoare_conj_pos hoare_kcomp hoare_while)*)
+
+
+(*
+lemma unfold_while:
+  assumes "`P \<longrightarrow> X`" "\<^bold>{P\<^bold>} (\<questiondown>X? ; Y)\<^sup>* ; Z \<^bold>{Q\<^bold>}"
+  shows "\<^bold>{P\<^bold>} Y ; (\<questiondown>X? ; Y)\<^sup>* ; Z \<^bold>{Q\<^bold>}"
+  using assms
+  by (metis (mono_tags, lifting) SEXP_def fbox_def fbox_kcomp predicate1D predicate1I)
+*)
+
+end
