Hybrid_Programs/Verification_Examples/Spring-Mass-Damper.thy
@@ -1,7 +1,0 @@
-theory SpringMassDamper
-
-imports
-  "Hybrid-Verification.Hybrid_Verification"
-begin
-  
-end
