Hybrid_Programs/Verification_Examples/WMR1.thy
@@ -1,0 +1,609 @@
+theory WMR1
+
+imports 
+  "Hybrid-Verification.Hybrid_Verification"
+  "Hoare_Help"
+begin
+
+lit_vars
+
+syntax "_do_while" :: "logic \<Rightarrow> logic \<Rightarrow> logic" ("DO _ WHILE _" [0,64] 64)
+translations "DO X WHILE T" => "X ; CONST while (T)\<^sub>e X"
+
+term "DO skip WHILE True"
+
+section \<open> Dataspace definition. \<close>
+
+text \<open> Version of the model where we do not consider torque. \<close>
+
+datatype STATE = 
+  Initial | SMoving | DMoving | Waiting | STurning | DTurning | 
+  DMovingJunction | DTurningJunction
+
+dataspace wmr_state = 
+  constants
+    \<comment> \<open> Robot d-model \<close>
+    LV     :: real
+    AV     :: real
+    \<comment> \<open> Robot p-model \<close>
+    RADIUS :: real
+    mass   :: real
+    WIDTH  :: real
+    LENGTH :: real
+    Cycle :: nat
+    TimeScale :: real
+    \<comment> \<open> Arena \<close>
+    size :: "real^3"
+    \<comment> \<open> Scenario: wheel inertias \<close>
+    lwI :: real
+    rwI :: real
+  assumes
+    non_zeros: "lwI > 0" "rwI > 0" "RADIUS > 0" "WIDTH > 0" "LENGTH > 0"
+  variables
+    \<comment> \<open> State machine variables and inputs/outputs \<close>
+    state     :: STATE
+    executing :: bool
+    obstacle  :: bool
+    MBC       :: nat
+    \<comment> \<open> Timer \<close>
+    timer     :: real
+    t         :: real (* global time *)
+    \<comment> \<open> P-model: torques and sensor input \<close>
+    IRVoltage :: real
+    IRDistance:: real
+    LMotorT   :: real
+    RMotorT   :: real
+    \<comment> \<open> Scenario mapping \<close>
+    robotPose :: "real^6"
+    (* How about local variables? I suppose for now need all of them visible/declared here. *)
+    \<comment> \<open> Scenario: robot position (px,py) and yaw (yw) \<close>
+    px :: "real"
+    py :: "real"
+    yw :: "real"
+    \<comment> \<open> Scenario: middle point between wheels (mx,my) \<close>
+    mx :: "real"
+    my :: "real"
+    \<comment> \<open> Scenario: wheel velocities \<close>
+    avLW :: "real"
+    avRW :: "real"
+
+dataspace wmr = wmr_state +
+  assumes
+    eq_IRVoltage_IRDistance: "$IRVoltage = 4*exp(-0.028784*$IRDistance)"
+  (* Not quite sure whether this is a good way to introduce algebraic equations. *)
+
+dataspace wmr_no_obstacle = wmr +
+  assumes
+    no_obstacle: "$IRDistance > - ln(3/4)/0.028784"
+
+context wmr
+begin
+
+lemma 
+  fixes IRD :: real
+  assumes "IRV = 4*exp(-0.028784*IRD)"
+  shows "IRD = - ln(IRV/4)/0.028784"
+  using assms by auto
+
+lemma IRDistance_no_detect:
+  fixes IRD :: real
+  assumes "4*exp(-0.028784*IRD) < K"
+  shows "IRD > - ln(K/4)/0.028784"
+proof -
+  have "exp(-0.028784*IRD) < K/4"
+    using assms by auto
+  then have "ln (exp(-0.028784*IRD)) < ln(K/4)"
+    by (metis dual_order.strict_trans exp_gt_zero exp_less_cancel_iff exp_ln)
+  then have "-0.028784*IRD < ln(K/4)"
+    by auto
+  then have "- IRD < ln(K/4)/0.028784"
+    by auto
+  then show ?thesis
+    by auto
+qed
+
+lemma IRDistance_no_detect_imp:
+  fixes IRD :: real
+  assumes "IRD > - ln(K/4)/0.028784" "K>0"
+  shows "4*exp(-0.028784*IRD) < K"
+proof -
+  have "-IRD < ln(K/4)/0.028784"
+    using assms by linarith
+  then have "-0.028784*IRD < ln(K/4)"
+    by auto
+  then have "exp(-0.028784*IRD) < exp(ln(K/4))"
+    by auto
+  then have "exp(-0.028784*IRD) < K/4"
+    using assms by auto
+  then show ?thesis by auto
+qed
+  
+lemma IRDistance_no_detect_iff:
+  fixes IRD :: real
+  assumes"K>0"
+  shows "IRD > - ln(K/4)/0.028784 \<longleftrightarrow> 4*exp(-0.028784*IRD) < K"
+  using IRDistance_no_detect IRDistance_no_detect_imp assms by blast
+  
+abbreviation "axisLength \<equiv> WIDTH+2*(RADIUS/4+0.5)"
+
+lemma avLW_avRW_dsl_dsr:
+  assumes "RADIUS > 0" "WIDTH > 0" "lv = RADIUS*(dsl+dsr)/2" "av = RADIUS*(dsl-dsr)/axisLength"
+  shows "dsl = (2*lv+av*axisLength)/(2*RADIUS)" "dsr = (2*lv-av*axisLength)/(2*RADIUS)"
+proof - 
+  obtain K1 K2 where K1_def:"K1 = 2*lv/RADIUS" and K2_def:"K2 = av*axisLength/RADIUS" by auto
+  from assms(1,3) K1_def have K1_eq:"K1 = dsl+dsr"
+    by force
+  from assms(1,2,4) K2_def have K2_eq: "K2 = dsl-dsr"
+    by auto
+
+  from K1_eq have dsl_eq_diff:"dsl = K1-dsr" by auto
+  then have dsr_K1_K2:"dsr = - (K2-K1)/2"
+    using K2_eq by simp
+  
+  then have dsl_K1_K2:"dsl = (K1+K2)/2"
+    using dsl_eq_diff by simp
+  also have "... = ((2*lv+av*axisLength)/RADIUS)/2"
+    by (simp add: K1_def K2_def add_divide_distrib)
+  also have "... = (2*lv+av*axisLength)/(2*RADIUS)"
+    using divide_divide_eq_left' by blast
+  then show "dsl = (2 * lv + av * axisLength) / (2 * RADIUS)"
+    using calculation by blast
+
+  then show "dsr = (2*lv-av*axisLength)/(2*RADIUS)"
+    by (metis K2_def dsl_K1_K2 dsr_K1_K2 diff_divide_distrib divide_divide_eq_left' minus_diff_eq mult.commute real_average_minus_second)
+qed
+
+text \<open> Platform operation mappings \<close>
+
+abbreviation "Move lv av \<equiv> avLW ::= (2*lv+av*axisLength)/(2*RADIUS) ; avRW ::= (2*lv-av*axisLength)/(2*RADIUS)"
+abbreviation "Stop \<equiv> avLW ::= 0 ; avRW ::= 0"
+
+(*abbreviation "exec P \<equiv> 
+  IF startexec \<and> \<not> endexec THEN endexec ::= True ; startexec ::= False ELSE
+  IF startexec \<and> endexec THEN endexec ::= False ; P ELSE skip"*)
+
+abbreviation "exec P \<equiv> 
+  IF executing THEN executing ::= False ELSE (executing ::= True ; P)"
+
+text \<open> The state machine is defined below in a style that lends itself to being executed N 
+       times till it reaches an exec. This helps with writing of the state machine. \<close>
+
+definition[simp]: "SimSMovement \<equiv> 
+  IF state = Initial THEN MBC ::= 0 ; state ::= SMoving ELSE
+  IF state = SMoving THEN Move LV 0 ; state ::= DMoving ELSE
+  IF state = DMoving THEN exec (state ::= DMovingJunction) ELSE 
+  IF state = DMovingJunction \<and> obstacle THEN exec (MBC ::= 0 ; Stop ; state ::= Waiting) ELSE
+  IF state = DMovingJunction \<and> \<not>obstacle THEN state ::= DMoving ELSE
+  IF state = Waiting THEN exec (state ::= STurning) ELSE
+  IF state = STurning THEN Move 0 AV ; state ::= DTurning ELSE
+  IF state = DTurning THEN exec (state ::= DTurningJunction) ELSE
+  IF state = DTurningJunction \<and> MBC < pi/AV THEN state ::= DTurning ELSE
+  IF state = DTurningJunction \<and> MBC \<ge> pi/AV THEN state ::= SMoving ELSE skip" 
+
+lemma simS1: "\<^bold>{state = Initial \<and> executing\<^bold>} SimSMovement \<^bold>{state = SMoving \<and> executing\<^bold>}"
+  by (hoare_wp_simp)
+
+lemma simS1': "\<^bold>{state = Initial \<and> executing\<^bold>} SimSMovement ; SimSMovement \<^bold>{state = DMoving \<and> executing\<^bold>}"
+  by (hoare_wp_simp)
+
+lemma simS1'': "\<^bold>{state = DMoving \<and> executing\<^bold>} SimSMovement \<^bold>{state = DMoving \<and> \<not>executing\<^bold>}"
+  by (hoare_wp_auto)
+
+lemma simS1''': "\<^bold>{state = Initial \<and> executing\<^bold>} SimSMovement ; SimSMovement ; SimSMovement \<^bold>{state = DMoving \<and> \<not> executing\<^bold>}"
+  by (hoare_wp_auto)
+
+(*lemma simS2: "\<^bold>{state = DMoving \<and> \<not> startexec \<and> endexec\<^bold>} SimSMovement \<^bold>{state = DMoving \<and> \<not> startexec \<and> endexec\<^bold>}"
+  by hoare_wp_auto
+
+text \<open> Checks that SimSMovement behaves as expected. \<close>
+
+lemma simS3: "\<^bold>{state = DMoving \<and> \<not> startexec \<and> endexec\<^bold>} SimSMovement\<^sup>* \<^bold>{state = DMoving \<and> \<not> startexec \<and> endexec\<^bold>}"
+  using hoare_kstar_inv simS2 by blast*)
+
+lemma simS4: "\<^bold>{True\<^bold>} (timer ::= y) \<^bold>{timer = y\<^bold>}"
+  by hoare_wp_auto
+
+lemma strengthen_pre:
+  assumes "\<^bold>{True\<^bold>} F \<^bold>{Q\<^bold>}"
+  shows "\<^bold>{Q\<^bold>} F \<^bold>{Q\<^bold>}"
+  using assms by auto
+
+text \<open> Therefore, we could have the following software controller. \<close>
+
+definition[simp]: "Init \<equiv> executing ::= True ; obstacle ::= False ; state ::= Initial"
+definition[simp]: "SendToSoftware \<equiv> IF IRVoltage \<ge> 3.0 THEN obstacle ::= True ELSE obstacle ::= False"
+definition[simp]: "Ctrl \<equiv> SendToSoftware ; DO SimSMovement WHILE executing ; timer ::= 0"
+
+section \<open> Platform and scenario modelling \<close>
+
+subsection \<open> Version 0: no torque, assumes instantaneous change in velocity and no obstacles. \<close>
+
+abbreviation 
+  "PSEvolution \<equiv> 
+  {yw` = (RADIUS/axisLength * avRW)-(RADIUS/axisLength * avLW),
+   mx` = (RADIUS/2 * cos(yw) * avLW)+(RADIUS/2 * cos(yw) * avRW),
+   my` = (RADIUS/2 * sin(yw) * avLW)+(RADIUS/2 * sin(yw) * avRW),
+   timer` = 1,
+   t` = 1
+  }"
+
+abbreviation "System0 \<equiv> Init ; Ctrl ; ((IF timer \<ge> TimeScale*Cycle THEN Ctrl ELSE skip) ; PSEvolution)\<^sup>*"
+
+text \<open> In the first case, we show that if no obstacles => only linear behaviour relevant. \<close>
+
+lemma PSE_no_yaw_change: "\<^bold>{avRW = avLW \<and> yw = yw\<^sub>0\<^bold>} PSEvolution \<^bold>{avRW = avLW \<and> yw = yw\<^sub>0\<^bold>}"
+  by (dInduct_mega)
+
+lemma PSE_linear_motion:
+  "\<^bold>{avLW = LV/RADIUS \<and> avRW = LV/RADIUS \<and> yw = yw\<^sub>0 \<and> mx = mx\<^sub>i + t*LV * cos(yw) \<and> my = my\<^sub>i + t*LV * sin(yw)\<^bold>}
+    PSEvolution
+   \<^bold>{avLW = LV/RADIUS \<and> avRW = LV/RADIUS \<and> yw = yw\<^sub>0 \<and> mx = mx\<^sub>i + t*LV * cos(yw) \<and> my = my\<^sub>i + t*LV * sin(yw)\<^bold>}"
+  apply (dInduct_mega)
+  using non_zeros(3) apply blast
+  apply (dInduct_mega)
+  using non_zeros(3) by blast
+
+text \<open> Below the angular version. Note that AV is clockwise, ie. a positive velocity spins clockwise,
+       whereas yaw is measured anti-clockwise, so a positive velocity decreases the angle. \<close>
+
+lemma PSE_angular_motion:
+  "\<^bold>{avLW = AV*axisLength/(2*RADIUS) \<and> avRW = -AV*axisLength/(2*RADIUS) \<and> yw = yw\<^sub>0 - timer*AV \<and> mx = mx\<^sub>i \<and> my = my\<^sub>i\<^bold>}
+    PSEvolution
+   \<^bold>{avLW = AV*axisLength/(2*RADIUS) \<and> avRW = -AV*axisLength/(2*RADIUS) \<and> yw = yw\<^sub>0 - timer*AV \<and> mx = mx\<^sub>i \<and> my = my\<^sub>i\<^bold>}"
+  apply (dInduct_mega)
+  using non_zeros apply force+
+  by (dInduct_mega)
+
+end
+
+context wmr_no_obstacle
+begin
+
+text \<open> What we really want to prove: overall, system moves linearly. \<close>
+
+lemma
+  "\<^bold>{yw = yw\<^sub>0 \<and> mx = mx\<^sub>i + timer*LV * cos(yw) \<and> my = my\<^sub>i + timer*LV * sin(yw)\<^bold>}
+    System0
+   \<^bold>{yw = yw\<^sub>0 \<and> mx = mx\<^sub>i + timer*LV * cos(yw) \<and> my = my\<^sub>i + timer*LV * sin(yw)\<^bold>}"
+  oops
+
+lemma SendToSoftware_spec:
+  "\<^bold>{IRVoltage < 3\<^bold>} SendToSoftware \<^bold>{ \<not> obstacle \<^bold>}"
+  by (hoare_wp_auto)
+
+lemma SimSMovement_DMoving_no_exe_obstacle_spec:
+  "\<^bold>{state = DMoving \<and> \<not> executing \<and> \<not> obstacle\<^bold>}
+   SimSMovement
+   \<^bold>{state = DMovingJunction \<and> executing\<^bold>}"
+  by hoare_wp_auto
+
+lemma
+  "\<^bold>{state = DMoving \<and> \<not> executing \<and> \<not> obstacle\<^bold>}
+   SimSMovement ; SimSMovement ; SimSMovement
+   \<^bold>{state = DMoving \<and> \<not> executing \<and> \<not> obstacle\<^bold>}"
+   by hoare_wp_auto
+
+lemma SimSMovement_obs_executing:
+  "\<^bold>{\<not> obstacle \<and> state \<notin> {Initial,SMoving,DMovingJunction,Waiting,STurning,DTurning,DTurningJunction} \<and> avLW = LV / RADIUS \<and> avRW = LV / RADIUS \<and> executing\<^bold>} 
+    SimSMovement
+   \<^bold>{\<not> obstacle \<and> state \<notin> {Initial,SMoving,DMovingJunction,Waiting,STurning,DTurning,DTurningJunction} \<and> avLW = LV / RADIUS \<and> avRW = LV / RADIUS\<^bold>}"
+  by hoare_wp_auto
+
+lemma SimSMovement_obs_executing':
+  "\<^bold>{\<not> obstacle \<and> state = DMovingJunction \<and> avLW = LV / RADIUS \<and> avRW = LV / RADIUS \<and> executing\<^bold>} 
+    SimSMovement
+   \<^bold>{\<not> obstacle \<and> state = DMoving \<and> avLW = LV / RADIUS \<and> avRW = LV / RADIUS \<and> executing\<^bold>}"
+  by hoare_wp_auto
+
+(* What I really need to show *)
+
+(* Take the following two *)
+
+lemma SimSMovement_DMoving_IF_executing:
+  "\<^bold>{\<not> obstacle \<and> state = DMoving \<and> avLW = LV / RADIUS \<and> avRW = LV / RADIUS \<and> \<not> executing\<^bold>} 
+    SimSMovement ; IF executing THEN SimSMovement ELSE skip
+   \<^bold>{\<not> obstacle \<and> state = DMoving \<and> avLW = LV / RADIUS \<and> avRW = LV / RADIUS \<and> executing\<^bold>}"
+  by hoare_wp_auto
+
+lemma SimSMovement_DMoving_executing_need:
+  "\<^bold>{\<not> obstacle \<and> state = DMoving \<and> avLW = LV / RADIUS \<and> avRW = LV / RADIUS \<and> executing\<^bold>} 
+    SimSMovement
+   \<^bold>{\<not> obstacle \<and> state = DMoving \<and> avLW = LV / RADIUS \<and> avRW = LV / RADIUS \<and> \<not> executing\<^bold>}"
+  by hoare_wp_auto
+
+lemma SimSMovement_obs_executing_need:
+  "\<^bold>{\<not> obstacle \<and> state = DMoving \<and> avLW = LV / RADIUS \<and> avRW = LV / RADIUS \<and> \<not> executing\<^bold>} 
+    DO SimSMovement WHILE executing
+   \<^bold>{\<not> obstacle \<and> state = DMoving \<and> avLW = LV / RADIUS \<and> avRW = LV / RADIUS \<and> \<not> executing\<^bold>}"
+proof -
+  have decomp:
+      "SimSMovement ; (WHILE executing DO SimSMovement) 
+       =
+       SimSMovement ; IF executing THEN SimSMovement ELSE skip ; (WHILE executing DO SimSMovement)
+      "
+      using WHILE_unroll_IF SimSMovement_DMoving_IF_executing
+      by (metis kcomp_assoc)
+
+    have a:"\<^bold>{\<not> obstacle \<and> state = DMoving \<and> avLW = LV / RADIUS \<and> avRW = LV / RADIUS \<and> \<not> executing\<^bold>} 
+          SimSMovement ; IF executing THEN SimSMovement ELSE skip
+          \<^bold>{\<not> obstacle \<and> state = DMoving \<and> avLW = LV / RADIUS \<and> avRW = LV / RADIUS \<and> executing\<^bold>}"
+      by hoare_wp_auto
+
+    have "\<^bold>{\<not> obstacle \<and> state = DMoving \<and> avLW = LV / RADIUS \<and> avRW = LV / RADIUS \<and> executing\<^bold>} 
+          SimSMovement 
+        \<^bold>{\<not> obstacle \<and> state = DMoving \<and> avLW = LV / RADIUS \<and> avRW = LV / RADIUS\<^bold>}"
+      by hoare_wp_auto
+    then have "\<^bold>{\<not> obstacle \<and> state = DMoving \<and> avLW = LV / RADIUS \<and> avRW = LV / RADIUS\<^bold>}
+          (WHILE executing DO SimSMovement) 
+          \<^bold>{\<not> executing \<and> \<not> obstacle \<and> state = DMoving \<and> avLW = LV / RADIUS \<and> avRW = LV / RADIUS\<^bold>}"
+      by (simp add: hoare_while)
+    then have b:"\<^bold>{\<not> obstacle \<and> state = DMoving \<and> avLW = LV / RADIUS \<and> avRW = LV / RADIUS \<and> executing\<^bold>}
+          (WHILE executing DO SimSMovement) 
+          \<^bold>{\<not> executing \<and> \<not> obstacle \<and> state = DMoving \<and> avLW = LV / RADIUS \<and> avRW = LV / RADIUS\<^bold>}"
+      using SEXP_def predicate1D by auto
+
+    from a b show ?thesis 
+      by (smt (verit, ccfv_threshold) SEXP_def decomp fbox_def hoare_kcomp le_fun_def)
+  (* This is not an invariant of WHILE _ DO _, but of DO _ WHILE _.
+     Proving it relies on being able to unroll the WHILE. *)
+  qed
+
+lemma SimSMovement_obs_not_executing_from_DMoving:
+  "\<^bold>{\<not> obstacle \<and> state = DMoving \<and> avLW = LV / RADIUS \<and> avRW = LV / RADIUS \<and> \<not> executing\<^bold>} 
+    SimSMovement
+   \<^bold>{\<not> obstacle \<and> state \<noteq> STurning \<and> avLW = LV / RADIUS \<and> avRW = LV / RADIUS \<and> executing\<^bold>}"
+  by hoare_wp_auto
+
+thm hoare_kcomp_inv_rhs
+thm hoare_kcomp
+
+lemma Ctrl_DMoving_inv:
+  "\<^bold>{IRVoltage < 3 \<and> state = DMoving \<and> avLW = LV/RADIUS \<and> avRW = LV/RADIUS \<and> \<not> executing\<^bold>}
+   Ctrl
+   \<^bold>{\<not> obstacle \<and> state = DMoving \<and> avLW = LV/RADIUS \<and> avRW = LV/RADIUS \<and> \<not> executing\<^bold>}"
+  unfolding Ctrl_def
+  apply (rule hoare_kcomp_inv_rhs)
+   apply (rule hoare_kcomp[where R="(\<not> obstacle \<and> state = DMoving \<and> avLW = LV/RADIUS \<and> avRW = LV/RADIUS \<and> \<not> executing )\<^sub>e"])
+    apply (hoare_wp_simp, simp del:SendToSoftware_def SimSMovement_def)
+  using SimSMovement_obs_executing_need apply metis 
+  by hoare_wp_simp
+
+named_theorems nmods
+
+
+
+thm nmods_seq
+thm nmods_while
+
+lemma nmods_set:
+  assumes "v \<in> s" "P nmods s"
+  shows "P nmods v"
+  using assms unfolding not_modifies_def by auto
+
+lemma nmods_set_expr:
+  assumes "v \<in> s" "P nmods s"
+  shows "P nmods F e"
+  using assms unfolding not_modifies_def by auto
+
+lemma nmods_subset:
+  assumes "v \<subseteq> s" "P nmods s"
+  shows "P nmods v"
+  using assms unfolding not_modifies_def by auto
+
+method nmods_auto = 
+  (auto intro: nmods_set nmods_subset)?;
+  ( 
+      (
+        (rule nmods_assign ; expr_simp)
+      | (rule nmods_if) 
+      | (rule nmods_while)
+      | (rule nmods_seq) 
+      | (rule nmods_assign) 
+      | (rule nmods_skip)
+      | (rule nmods_choice)
+      | (rule nmods_test)
+      | (rule nmods_star)
+      | (rule nmods_invariant ; (auto intro!: nmods_set nmods_subset nmods_subset)?)
+      | (simp only:nmods)
+    )
+  )+
+
+(* Q: Is there a better way to define a constant that has IRVoltage, IRDistance, etc? *)
+
+lemma SendToSoftware_nmods_IRVoltage [nmods]:
+  "SendToSoftware nmods {IRVoltage,avLW,avRW,mx,yx,yw,t}"
+  unfolding SendToSoftware_def
+  by nmods_auto
+
+lemma SimSMovement_nmods_IRVoltage [nmods]: 
+  "SimSMovement nmods {IRVoltage,mx,yx,yw,t}"
+  unfolding SimSMovement_def 
+  by nmods_auto
+
+lemma Ctrl_nmods [nmods]: 
+  "Ctrl nmods {IRVoltage,mx,yx,yw,t}"
+  unfolding Ctrl_def by nmods_auto
+
+lemma IF_Ctrl_Skip:
+  "(IF timer \<ge> TimeScale*Cycle THEN Ctrl ELSE skip) nmods {IRVoltage,mx,yx,yw,t}"
+  by nmods_auto
+
+lemma Ctrl_IF:
+  "\<^bold>{IRVoltage < 3 \<and> state = DMoving \<and> avLW = LV/RADIUS \<and> avRW = LV/RADIUS \<and> \<not> executing\<^bold>}
+   (IF timer \<ge> TimeScale*Cycle THEN Ctrl ELSE skip)
+   \<^bold>{IRVoltage < 3 \<and> state = DMoving \<and> avLW = LV/RADIUS \<and> avRW = LV/RADIUS \<and> \<not> executing\<^bold>}"
+proof -
+  have 
+    "\<^bold>{IRVoltage < 3 \<and> state = DMoving \<and> avLW = LV/RADIUS \<and> avRW = LV/RADIUS \<and> \<not> executing\<^bold>}
+     Ctrl
+     \<^bold>{\<not> obstacle \<and> state = DMoving \<and> avLW = LV/RADIUS \<and> avRW = LV/RADIUS \<and> \<not> executing\<^bold>}"
+    using Ctrl_DMoving_inv by blast
+  then have 
+    "\<^bold>{IRVoltage < 3 \<and> state = DMoving \<and> avLW = LV/RADIUS \<and> avRW = LV/RADIUS \<and> \<not> executing\<^bold>}
+     Ctrl
+     \<^bold>{state = DMoving \<and> avLW = LV/RADIUS \<and> avRW = LV/RADIUS \<and> \<not> executing\<^bold>}"
+    by (simp add: hoare_conj_pos)
+  then have 
+    "\<^bold>{state = DMoving \<and> avLW = LV/RADIUS \<and> avRW = LV/RADIUS \<and> \<not> executing \<and> IRVoltage < 3\<^bold>}
+     Ctrl
+     \<^bold>{state = DMoving \<and> avLW = LV/RADIUS \<and> avRW = LV/RADIUS \<and> \<not> executing\<^bold>}"
+    by auto
+  then have 
+    "\<^bold>{(state = DMoving \<and> avLW = LV/RADIUS \<and> avRW = LV/RADIUS \<and> \<not> executing) \<and> IRVoltage < 3\<^bold>}
+     Ctrl
+     \<^bold>{(state = DMoving \<and> avLW = LV/RADIUS \<and> avRW = LV/RADIUS \<and> \<not> executing) \<and> IRVoltage < 3\<^bold>}"
+    apply (rule_tac nmods_frame_law')
+    apply nmods_auto
+    by (smt (verit, del_insts) nmods_set SEXP_def fbox_def le_bool_def le_fun_def not_modifies_def)
+    (* FIXME: Introduce Hoare law for this *)
+  then have 
+    "\<^bold>{IRVoltage < 3 \<and> state = DMoving \<and> avLW = LV/RADIUS \<and> avRW = LV/RADIUS \<and> \<not> executing\<^bold>}
+     Ctrl
+     \<^bold>{IRVoltage < 3 \<and> state = DMoving \<and> avLW = LV/RADIUS \<and> avRW = LV/RADIUS \<and> \<not> executing\<^bold>}"
+    by (smt (verit) SEXP_def fbox_inv predicate1I)
+  then have
+    "\<^bold>{IRVoltage < 3 \<and> state = DMoving \<and> avLW = LV/RADIUS \<and> avRW = LV/RADIUS \<and> \<not> executing\<^bold>}
+     (IF timer \<ge> TimeScale*Cycle THEN Ctrl ELSE skip)
+     \<^bold>{IRVoltage < 3 \<and> state = DMoving \<and> avLW = LV/RADIUS \<and> avRW = LV/RADIUS \<and> \<not> executing\<^bold>}"
+    apply (rule hoare_if_then_else)
+    by (rule hoare_skip)
+  then show ?thesis .
+  (* Not sure whether this is sufficiently strong as an invariant *)
+qed
+
+lemma Ctrl_IF':
+  "\<^bold>{IRVoltage < 3 \<and> state = DMoving \<and> avLW = LV/RADIUS \<and> avRW = LV/RADIUS \<and> \<not> executing \<and> yw = yw\<^sub>0 \<and> mx = mx\<^sub>i + t*LV * cos(yw) \<and> my = my\<^sub>i + t*LV * sin(yw)\<^bold>}
+   (IF timer \<ge> TimeScale*Cycle THEN Ctrl ELSE skip)
+   \<^bold>{IRVoltage < 3 \<and> state = DMoving \<and> avLW = LV/RADIUS \<and> avRW = LV/RADIUS \<and> \<not> executing \<and> yw = yw\<^sub>0 \<and> mx = mx\<^sub>i + t*LV * cos(yw) \<and> my = my\<^sub>i + t*LV * sin(yw)\<^bold>}"
+proof -
+  have
+  "\<^bold>{(IRVoltage < 3 \<and> state = DMoving \<and> avLW = LV/RADIUS \<and> avRW = LV/RADIUS \<and> \<not> executing) \<and> yw = yw\<^sub>0 \<and> mx = mx\<^sub>i + t*LV * cos(yw) \<and> my = my\<^sub>i + t*LV * sin(yw)\<^bold>}
+   (IF timer \<ge> TimeScale*Cycle THEN Ctrl ELSE skip)
+   \<^bold>{(IRVoltage < 3 \<and> state = DMoving \<and> avLW = LV/RADIUS \<and> avRW = LV/RADIUS \<and> \<not> executing) \<and> yw = yw\<^sub>0 \<and> mx = mx\<^sub>i + t*LV * cos(yw) \<and> my = my\<^sub>i + t*LV * sin(yw)\<^bold>}"
+  apply (rule nmods_frame_law)
+   apply nmods_auto
+    using Ctrl_IF by blast
+  then show ?thesis
+    by presburger
+qed
+
+lemma PSEvolution_nmods [nmods]:
+  "PSEvolution nmods {state}"
+  by (auto intro!:closure, subst_eval)
+
+lemma PSE_linear_motion':
+  "\<^bold>{IRVoltage < 3 \<and> state = DMoving \<and> avLW = LV/RADIUS \<and> avRW = LV/RADIUS \<and> \<not> executing \<and> yw = yw\<^sub>0 \<and> mx = mx\<^sub>i + t*LV * cos(yw) \<and> my = my\<^sub>i + t*LV * sin(yw)\<^bold>}
+    PSEvolution
+   \<^bold>{IRVoltage < 3 \<and> state = DMoving \<and> avLW = LV/RADIUS \<and> avRW = LV/RADIUS \<and> \<not> executing \<and> yw = yw\<^sub>0 \<and> mx = mx\<^sub>i + t*LV * cos(yw) \<and> my = my\<^sub>i + t*LV * sin(yw)\<^bold>}"
+  apply (dInduct_mega)
+   apply (rule nmods_invariant) 
+   defer
+   apply (dInduct_mega)
+   apply (rule nmods_invariant) 
+    defer
+   apply (dInduct_mega)
+  using non_zeros(3) apply blast
+   apply (dInduct_mega)
+  using non_zeros(3) apply blast
+  by (auto intro!:closure, subst_eval, subst_eval)
+
+lemma Ctrl_IF_PSEvolution:
+  "\<^bold>{IRVoltage < 3 \<and> state = DMoving \<and> avLW = LV/RADIUS \<and> avRW = LV/RADIUS \<and> \<not> executing \<and> yw = yw\<^sub>0 \<and> mx = mx\<^sub>i + t*LV * cos(yw) \<and> my = my\<^sub>i + t*LV * sin(yw)\<^bold>}
+   (IF timer \<ge> TimeScale*Cycle THEN Ctrl ELSE skip) ; PSEvolution
+   \<^bold>{IRVoltage < 3 \<and> state = DMoving \<and> avLW = LV/RADIUS \<and> avRW = LV/RADIUS \<and> \<not> executing \<and> yw = yw\<^sub>0 \<and> mx = mx\<^sub>i + t*LV * cos(yw) \<and> my = my\<^sub>i + t*LV * sin(yw)\<^bold>}"
+  using Ctrl_IF' PSE_linear_motion' hoare_kcomp
+  by blast
+
+lemma Ctrl_IF_PSEvolution_iter:
+  "\<^bold>{IRVoltage < 3 \<and> state = DMoving \<and> avLW = LV/RADIUS \<and> avRW = LV/RADIUS \<and> \<not> executing \<and> yw = yw\<^sub>0 \<and> mx = mx\<^sub>i + t*LV * cos(yw) \<and> my = my\<^sub>i + t*LV * sin(yw)\<^bold>}
+   ((IF timer \<ge> TimeScale*Cycle THEN Ctrl ELSE skip) ; PSEvolution)\<^sup>*
+   \<^bold>{IRVoltage < 3 \<and> state = DMoving \<and> avLW = LV/RADIUS \<and> avRW = LV/RADIUS \<and> \<not> executing \<and> yw = yw\<^sub>0 \<and> mx = mx\<^sub>i + t*LV * cos(yw) \<and> my = my\<^sub>i + t*LV * sin(yw)\<^bold>}"
+  using Ctrl_IF_PSEvolution hoare_kstar_inv by blast
+
+lemma Ctrl_IF_PSEvolution_iter':
+  "\<^bold>{IRVoltage < 3 \<and> state = DMoving \<and> avLW = LV/RADIUS \<and> avRW = LV/RADIUS \<and> \<not> executing \<and> yw = yw\<^sub>0 \<and> mx = mx\<^sub>i + t*LV * cos(yw) \<and> my = my\<^sub>i + t*LV * sin(yw)\<^bold>}
+   ((IF timer \<ge> TimeScale*Cycle THEN Ctrl ELSE skip) ; PSEvolution)\<^sup>*
+   \<^bold>{yw = yw\<^sub>0 \<and> mx = mx\<^sub>i + t*LV * cos(yw) \<and> my = my\<^sub>i + t*LV * sin(yw)\<^bold>}"
+  apply (rule hoare_weaken_post[where Q="(IRVoltage < 3 \<and> state = DMoving \<and> avLW = LV/RADIUS \<and> avRW = LV/RADIUS \<and> \<not> executing)\<^sup>e"])
+  using Ctrl_IF_PSEvolution_iter 
+  by simp
+
+lemma SimSMovement_Initial_to_DMoving:
+  "\<^bold>{executing \<and> state = Initial\<^bold>} 
+   DO SimSMovement WHILE executing
+   \<^bold>{\<not> executing \<and> state = DMoving \<and> avLW = LV/RADIUS \<and> avRW = LV/RADIUS\<^bold>}"
+  apply (rule hoare_kcomp[where R="(executing \<and> state = SMoving)\<^sup>e"], hoare_wp_simp)
+  apply (rule hoare_while_unroll_kcomp[where Q="(state = DMoving \<and> avLW = LV/RADIUS \<and> avRW = LV/RADIUS \<and> executing)\<^sup>e"])
+   apply (hoare_wp_simp)
+  apply (rule hoare_while_unroll_kcomp[where Q="(state = DMoving \<and> avLW = LV/RADIUS \<and> avRW = LV/RADIUS)\<^sup>e"])
+   apply (hoare_wp_simp)
+  apply (rule hoare_while)
+  by (hoare_wp_simp)
+
+lemma Init_Ctrl:
+  "\<^bold>{True\<^bold>}
+   Init ; Ctrl
+   \<^bold>{state = DMoving \<and> avLW = LV/RADIUS \<and> avRW = LV/RADIUS \<and> \<not> executing\<^bold>}"
+  apply (rule hoare_kcomp[where R="(executing \<and> state = Initial)\<^sup>e"])
+   apply hoare_wp_simp
+  (*using IRDistance_no_detect_iff eq_IRVoltage_IRDistance no_obstacle apply simp*)
+  unfolding Ctrl_def
+  apply (rule hoare_kcomp[where R="(\<not> executing \<and> state = DMoving \<and> avLW = LV / RADIUS \<and> avRW = LV / RADIUS)\<^sup>e"])
+  defer
+   apply hoare_wp_simp
+  apply (rule hoare_kcomp[where R="(executing \<and> state = Initial)\<^sup>e"])
+  apply hoare_wp_simp
+  using SimSMovement_Initial_to_DMoving by blast
+
+lemma Init_yw_mx_my_Ctrl:
+  "\<^bold>{yw = yw\<^sub>0 \<and> mx = mx\<^sub>i + t*LV * cos(yw) \<and> my = my\<^sub>i + t*LV * sin(yw)\<^bold>}
+   Init ; Ctrl
+   \<^bold>{(state = DMoving \<and> avLW = LV/RADIUS \<and> avRW = LV/RADIUS \<and> \<not> executing) 
+    \<and> yw = yw\<^sub>0 \<and> mx = mx\<^sub>i + t*LV * cos(yw) \<and> my = my\<^sub>i + t*LV * sin(yw)\<^bold>}"
+  apply (rule hoare_weaken_pre_conj[where P="(True)\<^sup>e"], expr_simp)
+  apply (rule nmods_frame_law[where I="(yw = yw\<^sub>0 \<and> mx = mx\<^sub>i + t*LV * cos(yw) \<and> my = my\<^sub>i + t*LV * sin(yw))\<^sup>e"])
+   apply (nmods_auto)
+  using Init_Ctrl by blast
+
+lemma Init_yw_mx_my_Ctrl_Voltage:
+  "\<^bold>{yw = yw\<^sub>0 \<and> mx = mx\<^sub>i + t*LV * cos(yw) \<and> my = my\<^sub>i + t*LV * sin(yw)\<^bold>}
+   Init ; Ctrl
+   \<^bold>{IRVoltage < 3 \<and> state = DMoving \<and> avLW = LV/RADIUS \<and> avRW = LV/RADIUS \<and> \<not> executing
+    \<and> yw = yw\<^sub>0 \<and> mx = mx\<^sub>i + t*LV * cos(yw) \<and> my = my\<^sub>i + t*LV * sin(yw)\<^bold>}"
+  apply (rule hoare_strengthen_pos_universal)
+  using IRDistance_no_detect_iff eq_IRVoltage_IRDistance no_obstacle apply simp
+  using Init_yw_mx_my_Ctrl
+  by presburger
+
+theorem System0_behaviour:
+  "\<^bold>{yw = yw\<^sub>0 \<and> mx = mx\<^sub>i + t*LV * cos(yw) \<and> my = my\<^sub>i + t*LV * sin(yw)\<^bold>}
+    System0
+   \<^bold>{yw = yw\<^sub>0 \<and> mx = mx\<^sub>i + t*LV * cos(yw) \<and> my = my\<^sub>i + t*LV * sin(yw)\<^bold>}"
+  apply (rule hoare_kcomp[
+        where R="(IRVoltage < 3 \<and> state = DMoving \<and> avLW = LV/RADIUS \<and> avRW = LV/RADIUS \<and> \<not> executing
+    \<and> yw = yw\<^sub>0 \<and> mx = mx\<^sub>i + t*LV * cos(yw) \<and> my = my\<^sub>i + t*LV * sin(yw))\<^sup>e"])
+  using Init_yw_mx_my_Ctrl_Voltage apply blast
+  using Ctrl_IF_PSEvolution_iter' by blast
+
+lemma "\<^bold>{P\<^bold>} SendToSoftware \<^bold>{P \<and> \<not>obstacle\<^bold>}"
+  apply (hoare_wp_auto)
+  using no_obstacle IRDistance_no_detect_iff eq_IRVoltage_IRDistance
+  by (metis linorder_not_less zero_less_numeral)
+
+lemma SimSMovement_maintain_linear_motion: 
+  "\<^bold>{\<not> obstacle \<and> state \<noteq> STurning \<and> avLW = avRW\<^bold>}
+   SimSMovement
+   \<^bold>{\<not> obstacle \<and> avLW = avRW\<^bold>}"
+  by (hoare_wp_simp)
+
+lemma unfold_while:
+  assumes "`P \<longrightarrow> X`" "\<^bold>{P\<^bold>} (\<questiondown>X? ; Y)\<^sup>* ; Z \<^bold>{Q\<^bold>}"
+  shows "\<^bold>{P\<^bold>} Y ; (\<questiondown>X? ; Y)\<^sup>* ; Z \<^bold>{Q\<^bold>}"
+  using assms 
+  by (metis (mono_tags, lifting) SEXP_def fbox_def fbox_kcomp predicate1D predicate1I)
+  
+subsection \<open> Version with torque, no instantaneous change in velocity. \<close>
+
+end
+
+end
